proof/refine/ARM/Refine.thy
@@ -647,7 +647,7 @@ lemma entry_corres:
             apply (simp add: tcb_relation_def arch_tcb_relation_def
                              arch_tcb_context_set_def atcbContextSet_def)
            apply (clarsimp simp: tcb_cap_cases_def)
-          apply (clarsimp simp: tcb_cte_cases_def)
+          apply (clarsimp simp: tcb_cte_cases_def tcb_cte_cases_neqs)
          apply (simp add: exst_same_def)
         apply (rule corres_split[OF kernel_corres])
           apply (rule corres_split_eqr[OF getCurThread_corres])
